update

UnitProJ/expressOS/Fall2015/INode-delRegion.dfy
@@ -634,6 +634,15 @@ nd in ndSet
 }
 
 
+predicate delSeqHelperLemma(oldList:seq<INode>, oldFp:set<INode>, oldHdFp:set<INode>, hd:INode,newList:seq<INode>, newFp:set<INode>, newHdFp:set<INode>, fstNd:INode)
+	requires forall nd:: nd in oldList && nd in oldFp ==> nd in oldHdFp - {hd};
+	requires oldList == [fstNd] + newList &&
+		oldFp == newFp + {fstNd} &&
+		oldHdFp == newHdFp + {fstNd};
+		
+	reads oldList, oldFp, oldHdFp, hd, newList, newFp, newHdFp;
+	ensures forall nd:: nd in newList && nd in newFp ==> nd in newHdFp - {hd};
+{true}
 
 method delSeqOfNd(ndList:seq<INode>)
 	requires valid();
@@ -656,6 +665,9 @@ method delSeqOfNd(ndList:seq<INode>)
 	assert |ndList| == 1 ==> forall nd :: nd in ndList ==> nd == ndList[0];
 
 	assert footprint == old(footprint) - {ndList[0]};
+	assert head.footprint == old(head.footprint) - {ndList[0]};
+
+	assert delSeqHelperLemma(ndList, old(footprint), old(head.footprint), head, ndList[1..], footprint, head.footprint, ndList[0]);
 	
 delSeqOfNd(ndList[1..]);
 assert forall nd :: nd in ndList[1..] ==> nd !in footprint;
