UnitProJ/expressOS/Fall2015/flycheck_INode-delRegion.dfy
@@ -586,6 +586,7 @@ ensures spine == old(spine) - {delNd};
 //new
 ensures delNd != null && delNd.Valid();
 ensures delNd.footprint == old(delNd.footprint);
+ensures head.footprint == old(head.footprint) - {delNd};
 {
    delNd := head.delete(index+1);
 
@@ -609,7 +610,7 @@ method delNd(tarNd:INode)
 	modifies footprint;
 	ensures valid();
 	ensures footprint == old(footprint) - {tarNd};
-	
+	ensures head.footprint == old(head.footprint) - {tarNd};
 
 	//new
 	ensures tarNd.footprint == old(tarNd.footprint); 
@@ -633,6 +634,15 @@ nd in ndSet
 }
 
 
+predicate delSeqHelperLemma(oldList:seq<INode>, oldFp:set<INode>, oldHdFp:set<INode>, hd:INode,newList:seq<INode>, newFp:set<INode>, newHdFp:set<INode>, fstNd:INode)
+	requires forall nd:: nd in oldList && nd in oldFp ==> nd in oldHdFp - {hd};
+	requires oldList == [fstNd] + newList &&
+		oldFp == newFp + {fstNd} &&
+		oldHdFp == newHdFp + {fstNd};
+		
+	reads oldList, oldFp, oldHdFp, hd, newList, newFp, newHdFp;
+	ensures forall nd:: nd in newList && nd in newFp ==> nd in newHdFp - {hd};
+{true}
 
 method delSeqOfNd(ndList:seq<INode>)
 	requires valid();
@@ -655,7 +665,7 @@ method delSeqOfNd(ndList:seq<INode>)
 	assert |ndList| == 1 ==> forall nd :: nd in ndList ==> nd == ndList[0];
 
 	assert footprint == old(footprint) - {ndList[0]};
-	
+	assert head.footprint == old(head.footprint) - {ndList[0]};
 delSeqOfNd(ndList[1..]);
 assert forall nd :: nd in ndList[1..] ==> nd !in footprint;
 assert forall nd :: nd in ndList ==> nd !in footprint;
